sorry free :)

Projects/Wuethrich/List/Zip.lean
@@ -11,7 +11,7 @@ namespace List
 @[simp] theorem zipWith3_nil_left  : zipWith3 f [] bs cs = [] := rfl
 @[simp] theorem zipWith3_nil_middle : zipWith3 f as [] cs = [] := by simp [zipWith3]
 @[simp] theorem zipWith3_nil_right: zipWith3 f as bs [] = [] := by simp [zipWith3]
-@[simp] theorem zipWith3_cons_cons : zipWith3 f (a :: as) (b :: bs) (c :: cs) = f a b c :: zipWith3 f as bs cs := rfl
+@[simp] theorem zipWith3_cons_cons_cons : zipWith3 f (a :: as) (b :: bs) (c :: cs) = f a b c :: zipWith3 f as bs cs := rfl
 
 @[simp, grind =] theorem length_zipWith3 {f : α → β → γ → δ} {l₁ : List α} {l₂ : List β} {l₃  : List γ} :
     length (zipWith3 f l₁ l₂ l₃) = min (min (length l₁) (length l₂)) (length l₃) := by
@@ -53,3 +53,60 @@ theorem getElem_zipWith3 {f : α → β → γ → δ} {l₁ : List α} {l₂ : 
   rw [← Option.some_inj, ← getElem?_eq_getElem, getElem?_zipWith3_eq_some]
   simp only [length_zipWith3, Nat.min_assoc, lt_inf_iff] at h
   simp_all only [getElem?_pos, Option.some.injEq, exists_and_left, ↓existsAndEq, true_and, exists_eq_left']
+
+@[simp, grind =]
+theorem map_zipWith3 {ε : Type _} {f : δ → ε} {g : α → β → γ → δ}
+    {l₁ : List α} {l₂ : List β} {l₃ : List γ} :
+    map f (zipWith3 g l₁ l₂ l₃) = zipWith3 (fun x y z => f (g x y z)) l₁ l₂ l₃ := by
+  induction l₁ generalizing l₂ l₃ with
+  | nil => simp
+  | cons hd tl hl =>
+    cases l₂
+    · simp
+    · cases l₃
+      · simp
+      · simp [hl]
+
+
+universe u v w x y
+variable {m : Type u → Type v}
+variable {α : Type w} {β : Type x} {γ : Type y} {δ : Type u}
+
+@[inline, expose]
+def zipWith3M [Monad m] (f : α → β → γ → m δ) (as : List α) (bs : List β) (cs : List γ) : m (List δ) :=
+  let rec @[specialize] loop
+    | a::as, b::bs, c::cs, acc => do loop as bs cs (acc.push (← f a b c))
+    | _, _, _, acc => pure acc.toList
+  loop as bs cs #[]
+
+@[expose]
+def zipWith3M' [Monad m] (f : α → β → γ → m δ) : (xs : List α) → (ys : List β) → (zs : List γ) → m (List δ)
+  | x::xs, y::ys, z::zs => do
+    let w ← f x y z
+    let ws ← zipWith3M' f xs ys zs
+    pure (w :: ws)
+  | _, _, _ => pure []
+
+@[grind =]
+theorem zipWith3M'_eq_zipWith3M [Monad m] [LawfulMonad m]
+    {f : α → β → γ → m δ} {l₁ : List α} {l₂ : List β} {l₃ : List γ} :
+    zipWith3M' f l₁ l₂ l₃ = zipWith3M f l₁ l₂ l₃ := by
+  simp [zipWith3M, go l₁ l₂ l₃ #[]]
+where
+  go l₁ l₂ l₃ acc :
+    zipWith3M.loop f l₁ l₂ l₃ acc = return acc.toList ++ (← zipWith3M' f l₁ l₂ l₃) := by
+    fun_induction zipWith3M.loop <;> simp [zipWith3M', *]
+
+@[simp, grind =]
+theorem zipWith3M'_eq_mapM_id_zipWith [Monad m] [LawfulMonad m] {f : α → β → γ → m δ} {as : List α} {bs : List β} {cs : List γ} :
+    zipWith3M' f as bs cs = mapM id (zipWith3 f as bs cs) := by
+  fun_induction zipWith3M' <;> simp [zipWith3, *]
+
+variable {as : List α} {bs : List β} {cs : List γ} {a : α} {b : β} {c : γ}
+
+@[simp, grind =] theorem zipWith3M_nil_left [Monad m] {f : α → β → γ → m δ}  : zipWith3M f [] bs cs = pure (f := m) [] := rfl
+@[simp, grind =] theorem zipWith3M_nil_middle [Monad m] {f : α → β → γ → m δ}  : zipWith3M f as [] cs = pure (f := m) [] := by simp only [zipWith3M, zipWith3M.loop]
+@[simp, grind =] theorem zipWith3M_nil_right [Monad m] {f : α → β → γ → m δ}  : zipWith3M f as bs [] = pure (f := m) [] := by simp only [zipWith3M, zipWith3M.loop]
+@[simp, grind =] theorem zipWith3M_cons_cons_cons [Monad m] [LawfulMonad m] {f : α → β → γ → m δ} {as : List α} {bs : List β} {cs : List γ}  :
+    zipWith3M f (a :: as) (b :: bs) (c :: cs) = do return (← f a b c) :: (← zipWith3M f as bs cs) := by
+  simp [← zipWith3M'_eq_zipWith3M]
