Projects/Wuethrich/List/toArray.lean
@@ -1,11 +1,55 @@
 import Projects.Wuethrich.Array.Basic
+import Projects.Wuethrich.List.Zip
 
-variable {α β γ δ : Type*}
+universe u v w
+variable {α : Type u} {δ : Type v} {β γ : Type*}
 
 namespace List
+
+open Array
+
+theorem zipWith3MAux_toArray_succ {m : Type v → Type w} [Monad m]
+    (as : List α) (bs : List β) (cs : List γ) (f : α → β → γ → m δ) (i : Nat) (xs : Array δ) :
+    zipWith3MAux as.toArray bs.toArray cs.toArray f (i + 1) xs =
+      zipWith3MAux as.tail.toArray bs.tail.toArray cs.tail.toArray f i xs := by
+  rw [zipWith3MAux]
+  conv => rhs; rw [zipWith3MAux]
+  simp only [size_toArray, getElem_toArray, length_tail, getElem_tail]
+  split <;> rename_i h₁
+  · split <;> rename_i h₂
+    · split <;> rename_i h₃
+      · rw [dif_pos (by omega), dif_pos (by omega), dif_pos (by omega)]
+        simp only [zipWith3MAux_toArray_succ as bs cs f (i+1)]
+      · rw [dif_pos (by omega), dif_pos (by omega)]
+        rw [dif_neg (by omega)]
+    · rw [dif_pos (by omega)]
+      rw [dif_neg (by omega)]
+  · rw [dif_neg (by omega)]
+
+
+theorem zipWith3MAux_toArray_succ' {m : Type v → Type w} [Monad m]
+    (as : List α) (bs : List β) (cs : List γ)
+    (f : α → β → γ → m δ) (i : Nat) (xs : Array δ) :
+    zipWith3MAux as.toArray bs.toArray cs.toArray f (i + 1) xs =
+      zipWith3MAux (as.drop (i+1)).toArray (bs.drop (i+1)).toArray (cs.drop (i+1)).toArray f 0 xs := by
+  induction i generalizing as bs cs xs with
+  | zero => simp [zipWith3MAux_toArray_succ]
+  | succ i ih =>
+    rw [zipWith3MAux_toArray_succ, ih]
+    simp
+
+theorem zipWith3MAux_toArray_zero {m : Type v → Type w} [Monad m] [LawfulMonad m] (f : α → β → γ → m δ) (as : List α) (bs : List β) (cs : List γ) (xs : Array δ) :
+    Array.zipWith3MAux as.toArray bs.toArray cs.toArray f 0 xs = do return xs ++ (← List.zipWith3M f as bs cs).toArray := by
+  rw [Array.zipWith3MAux]
+  match as, bs, cs with
+  | [], _, _ => simp
+  | _, [], _ => simp
+  | _, _, [] => simp
+  | a :: as, b :: bs, c :: cs =>
+    simp [zipWith3MAux_toArray_succ', zipWith3MAux_toArray_zero]
+
 
 @[simp, grind =] theorem zipWith3_toArray (as : List α) (bs : List β) (cs : List γ) (f : α → β → γ → δ) :
     Array.zipWith3 f as.toArray bs.toArray cs.toArray = (List.zipWith3 f as bs cs).toArray := by
   rw [Array.zipWith3]
-  --simp [zipWithMAux_toArray_zero, ← zipWithM'_eq_zipWithM]
-  sorry
+  simp [zipWith3MAux_toArray_zero, ← zipWith3M'_eq_zipWith3M]
